ironfleet/src/Dafny/Distributed/Protocol/RSL/FailureProof/Phase2Proof_helper.i.dfy
@@ -32,7 +32,6 @@ lemma AlwaysInvariant_Maintained(ts:TimestampedRslState, ts':TimestampedRslState
     requires RslPerfInvariant(ts, opn)
     ensures AlwaysInvariant(ts')
 {
-
     assert ts'.t_replicas[1].v.replica.proposer.request_queue == [];
     assert forall pkt | pkt in ts'.t_replicas[1].v.replica.proposer.received_1b_packets && pkt.msg.RslMessage_1b? :: forall op | op in pkt.msg.votes :: RequestBatchSrcInClientIds(ts', pkt.msg.votes[op].max_val);
     forall pkt | pkt in ts'.undeliveredPackets && pkt.msg.v.RslMessage_2a? 
@@ -43,4 +42,30 @@ lemma AlwaysInvariant_Maintained(ts:TimestampedRslState, ts':TimestampedRslState
     {}
 }
 
+
+lemma Before2a_to_After2a(ts:TimestampedRslState, ts':TimestampedRslState, opn:OperationNumber, tios:seq<TimestampedLIoOp<NodeIdentity, RslMessage>>) 
+    requires RslAssumption(ts) && RslConsistency(ts)
+    requires RslAssumption(ts') && RslConsistency(ts')
+    requires PacketsBallotInvariant(ts) && PacketsBallotInvariant(ts')
+    requires TimestampedRslNext(ts, ts')
+    requires !TimestampedRslNextEnvironment(ts, ts')
+    requires TimestampedRslNextOneReplica(ts, ts', 1, tios);
+    requires RslPerfInvariant(ts, opn)
+    requires Before_2a_Sent_Invariant(ts, opn);
+    ensures After_2a_Sent_Invariant(ts', opn);
+{
+    var s, s', ios := UntimestampRslState(ts), UntimestampRslState(ts'), UntagLIoOpSeq(tios);
+    var r, r' := s.replicas[1].replica, s'.replicas[1].replica;
+    var sent_packets := ExtractSentPacketsFromIos(ios);
+    var v :| 
+        (&& LValIsHighestNumberedProposal(v, r.proposer.received_1b_packets, opn)
+         && LBroadcastToEveryone(r.proposer.constants.all.config, r.proposer.constants.my_index, RslMessage_2a(r.proposer.max_ballot_i_sent_1a, opn, v), sent_packets)
+    );
+    assert |sent_packets| > 0;
+    var m := RslMessage_2a(Ballot(1, 1), opn, v);
+    assert sent_packets[0] == LPacket(r.proposer.constants.all.config.replica_ids[0], r.proposer.constants.all.config.replica_ids[1], m);
+    var pkt_witness := sent_packets[0];
+    assert LIoOpSend(pkt_witness) in ios;
+    assert After_2a_Sent_Invariant(ts', opn);
+}
 }
